chore: bump to v4.21.0 & update dependencies + remove non-terminal `simp`s

Veil/Frontend/DSL/Action/Semantics/WP.lean
@@ -15,6 +15,18 @@ def VeilExecM.assert (p : Prop) [Decidable p] (ex : ExId) : VeilExecM m ρ σ Un
 def VeilM.assert (p : Prop) [Decidable p] (ex : ExId) : VeilM m ρ σ Unit := do
   liftM (@VeilExecM.assert m ρ σ p _ ex)
 
+/-- We require the predicate to be `Decidable`, even though `assume`
+does not, in order to collect the appropriate instances needed for
+execution. -/
+def VeilM.assume (p : Prop) [Decidable p] : VeilM m ρ σ PUnit := do
+  MonadNonDet.assume p
+
+/-- We require the predicate to be `Decidable`, even though `assume`
+does not, in order to collect the appropriate instances needed for
+execution. -/
+def VeilM.pickSuchThat (τ : Type) (p : τ → Prop) [∀ x, Decidable (p x)] : VeilM m ρ σ τ := do
+  MonadNonDet.pickSuchThat τ p
+
 def VeilM.require (p : Prop) [Decidable p] (ex : ExId) : VeilM m ρ σ Unit := do
   match m with
   | .internal => VeilM.assert p ex
@@ -61,10 +73,11 @@ lemma VeilExecM.wp_assert (p : Prop) {_ : Decidable p} (ex : ExId) :
   wp (@VeilExecM.assert m ρ σ p _ ex) post = fun r s => if p then post () r s else hd ex := by
   simp [VeilExecM.assert]; split
   { simp [wp_pure] }
-  simp [throw, throwThe, ReaderT.instMonadExceptOf, StateT.instMonadExceptOf]
+  simp only [throw, throwThe, ReaderT.instMonadExceptOf, StateT.instMonadExceptOf,
+    Function.comp_apply]
   have : ∀ (α σ : Type) (m : Type -> Type) [Monad m], StateT.lift (σ := σ) (α := α) (m := m) = liftM := by
     simp [liftM, monadLift, StateT.instMonadLift]
-  simp [this, MAlgLift.wp_lift]; erw [ExceptT.wp_throw]
+  simp only [this, MAlgLift.wp_lift, lift_cont_eq]; erw [ExceptT.wp_throw]
   simp [loomLogicSimp]
 
 @[wpSimp]
@@ -75,66 +88,71 @@ lemma VeilM.wp_assert (p : Prop) {_ : Decidable p} (ex : ExId) :
 @[wpSimp]
 lemma VeilM.wp_get {_ : IsSubStateOf σₛ σ} :
   wp (get : VeilM m ρ σ σₛ) post = fun r s => post (getFrom s) r s := by
-  simp [get, getThe, MonadStateOf.get, MAlgLift.wp_lift]; ext
+  simp only [get, getThe, MonadStateOf.get, MAlgLift.wp_lift, lift_cont_eq, monadLift_self]; ext
   erw [StateT.wp_get]
 
 @[wpSimp low]
 lemma VeilM.wp_get' :
   wp (get : VeilM m ρ σ σ) post = fun r s => post s r s := by
-  simp [get, getThe, MonadStateOf.get, MAlgLift.wp_lift]; ext
+  simp only [get, getThe, MonadStateOf.get, MAlgLift.wp_lift, lift_cont_eq, monadLift_self]; ext
   erw [StateT.wp_get]
 
 @[wpSimp]
 lemma VeilM.wp_set {_ : IsSubStateOf σₛ σ} :
   wp (set s': VeilM m ρ σ Unit) post = fun r s => post () r (setIn s' s) := by
-  simp [set, MAlgLift.wp_lift, modify, modifyGet, MonadStateOf.modifyGet]; ext
+  simp only [set, modify, modifyGet, MonadStateOf.modifyGet, MAlgLift.wp_lift, lift_cont_eq,
+    monadLift_self]; ext
   erw [StateT.wp_modifyGet]
 
 @[wpSimp low]
 lemma VeilM.wp_set' :
   wp (set s': VeilM m ρ σ Unit) post = fun r _s => post () r s' := by
-  simp [set, MAlgLift.wp_lift, modify, modifyGet, MonadStateOf.modifyGet]; ext
+  simp only [set, modify, modifyGet, MonadStateOf.modifyGet, MAlgLift.wp_lift, lift_cont_eq,
+    monadLift_self]; ext
   erw [StateT.wp_modifyGet]; rfl
 
 @[wpSimp]
 lemma VeilM.wp_modifyGet {_ : IsSubStateOf σₛ σ} :
   wp (modifyGet f : VeilM m ρ σ α) post = fun r s => post (f (getFrom s)).1 r (setIn (f (getFrom s)).2 s) := by
-  simp [modifyGet, MonadStateOf.modifyGet, MAlgLift.wp_lift]; ext
+  simp only [modifyGet, MonadStateOf.modifyGet, MAlgLift.wp_lift, lift_cont_eq, monadLift_self]; ext
   erw [StateT.wp_modifyGet]
 
 @[wpSimp low]
 lemma VeilM.wp_modifyGet' :
   wp (modifyGet f : VeilM m ρ σ α) post = fun r s => post (f s).1 r (f s).2 := by
-  simp [modifyGet, MonadStateOf.modifyGet, MAlgLift.wp_lift]; ext
+  simp only [modifyGet, MonadStateOf.modifyGet, MAlgLift.wp_lift, lift_cont_eq, monadLift_self]; ext
   erw [StateT.wp_modifyGet]; rfl
 
 @[wpSimp]
 lemma VeilM.wp_read {_ : IsSubReaderOf ρₛ ρ} :
   wp (read : VeilM m ρ σ ρₛ) post = fun r s => post (readFrom r) r s := by
-  simp [read, getThe, MonadReaderOf.read, readThe, MAlgLift.wp_lift]; ext
+  simp only [read, readThe, MonadReaderOf.read, MAlgLift.wp_lift, monadLift_self]; ext
   erw [ReaderT.wp_read]
 
 @[wpSimp low]
 lemma VeilM.wp_read' :
   wp (read : VeilM m ρ σ ρ) post = fun r s => post r r s := by
-  simp [read, getThe, MonadReaderOf.read, readThe, MAlgLift.wp_lift]; ext
+  simp only [read, readThe, MonadReaderOf.read, MAlgLift.wp_lift, monadLift_self]; ext
   erw [ReaderT.wp_read]
 
 @[wpSimp]
 lemma VeilM.wp_pick :
   wp (pick τ : VeilM m ρ σ τ) post = fun r s => ∀ t, post t r s := by
-  simp [MonadNonDet.wp_pick, loomLogicSimp, himp, iInf, sInf]; aesop
+  simp only [MonadNonDet.wp_pick, iInf, sInf, Set.mem_range, eq_iff_iff, Subtype.exists,
+    exists_prop, exists_exists_eq_and, forall_exists_index]; aesop
 
 @[wpSimp]
-lemma VeilM.wp_pickSuchThat :
-  wp (pickSuchThat τ p : VeilM m ρ σ τ) post = fun r s => ∀ t, p t -> post t r s := by
-  simp [MonadNonDet.wp_pickSuchThat, loomLogicSimp, himp, iInf, sInf]; aesop
+lemma VeilM.wp_pickSuchThat {m : Mode} {ρ σ τ : Type} {p : τ → Prop} {_ : ∀ x, Decidable (p x)} {post : τ → ρ → σ → Prop} :
+  wp (VeilM.pickSuchThat τ p : VeilM m ρ σ τ) post = fun r s => ∀ t, p t -> post t r s := by
+  simp only [VeilM.pickSuchThat, MonadNonDet.wp_pickSuchThat, iInf, sInf, himpE, himpPureE, Set.mem_range, eq_iff_iff,
+    Subtype.exists, pureE, purePropE, exists_prop, exists_exists_eq_and, forall_exists_index]
+  aesop
 
 @[wpSimp]
 lemma VeilM.wp_if [Decidable p] :
   wp (if p then a else b : VeilM m ρ σ τ) post =
   if p then wp a post else wp b post := by
-  split_ifs <;> simp
+  split_ifs <;> simp only
 
 attribute [wpSimp] wp_pure wp_bind wp_map wp_bind
 
